src/assignments/hw5_expr_langs/arith_expr.lean
@@ -1,0 +1,60 @@
+-- SYNTAX
+
+-- Variables ADT
+
+-- data type
+inductive nat_var 
+| Δ (n : ℕ)
+
+open nat_var
+
+-- operations
+def nat_var_eq : nat_var → nat_var → bool
+| (Δ n) (Δ m) :=  n = m   -- coercion here
+
+-- notationss
+notation e1 = e2 := nat_var_eq e1 e2
+
+-- expression ADT
+
+-- data type
+inductive nat_expr : Type
+| lit (n : nat)
+| var (v : nat_var) 
+| dec (e : nat_expr) 
+| inc (e : nat_expr) 
+| add (e1 e2 : nat_expr)
+
+open nat_expr
+
+-- notations
+notation `[`n`]` := lit n     -- we overload []
+notation `[`v`]` := var v     -- there and here
+postfix `++` :=  inc
+notation e1 + e2 := add e1 e2
+
+-- interpretation ADT
+
+-- type
+def nat_var_interp := (nat_var → nat)
+
+-- operations
+def override : 
+  nat_var_interp → 
+  nat_var → 
+  nat → 
+  nat_var_interp :=
+λ i v n,
+  λ x, 
+    if (nat_var_eq x v) 
+    then n 
+    else i x
+
+-- semantics : assign nat value to any expr given interp
+
+def eval : nat_expr → nat_var_interp → nat
+| (lit n) _ := n
+| (var v) i := i v
+| (dec e) i := (eval e i) - 1
+| (inc e) i := (eval e i) + 1
+| (add e1 e2) i := (eval e1 i) + (eval e2 i)
