src/assignments/hw5_expr_langs/arith_expr/eval.lean
@@ -1,0 +1,13 @@
+import .expr 
+import .interp
+
+-- semantics : assign nat value to any expr given interp
+
+open nat_expr
+
+def eval : nat_expr → nat_var_interp → nat
+| (lit n) _ := n
+| (var v) i := i v
+| (dec e) i := (eval e i) - 1
+| (inc e) i := (eval e i) + 1
+| (add e1 e2) i := (eval e1 i) + (eval e2 i)
