src/assignments/hw5_expr_langs/arith_expr/var.lean
@@ -1,0 +1,16 @@
+-- SYNTAX
+
+-- Variables ADT
+
+-- data type
+inductive nat_var 
+| Δ (n : ℕ)
+
+open nat_var
+
+-- operations
+def nat_var_eq : nat_var → nat_var → bool
+| (Δ n) (Δ m) :=  n = m   -- coercion here
+
+-- notationss
+notation e1 = e2 := nat_var_eq e1 e2
