src/assignments/hw5_expr_langs/bool_expr/bool_expr.lean
@@ -1,0 +1,211 @@
+import .bool
+import .arith_lang
+
+namespace arith 
+
+open arith
+open hidden
+
+-- DATA TYPE
+
+/-
+inductive bool_var 
+| X
+| Y 
+| Z
+-/
+
+inductive bool_var 
+| V (n : ℕ)
+
+open bool_var
+
+-- Test
+def X := V 0
+def Y := V 1
+def Z := V 2
+
+inductive bool_lang : Type
+| TT : bool_lang
+| FF : bool_lang
+| var (v : bool_var) : bool_lang
+| conj (e1 e2 : bool_lang) : bool_lang
+| disj (e1 e2 : bool_lang) : bool_lang
+| neg (e : bool_lang)
+| eql (e1 e2 : nt_lang)
+
+
+-- REFACTOR INTO TEST FILE
+open bool_lang
+def be1 := TT
+def be2 := FF
+def ve1 := var X
+def be3 := conj be1 be2
+def be4 := neg be3
+
+def var_interp_1 : bool_var → boo
+| v := boo.tt
+
+/-
+def var_interp_2 : bool_var → boo
+| X := tt
+| Y := ff
+| Z := tt
+-/
+
+def var_interp_2 : bool_var → boo
+| (V 0) := tt
+| (V 1) := ff
+| (V 2) := tt
+| _ := tt
+
+-- OPERATIONS
+def eval : bool_lang → (bool_var → boo) → boo
+| TT _ := tt
+| FF _ := ff
+| (var v) i := i v
+| (conj e1 e2) i := and (eval e1 i) (eval e2 i)
+| (disj e1 e2) i := or (eval e1 i) (eval e2 i)
+| (neg e) i := not (eval e i)
+| (eql e1 e2) := _ -- evaluate e1, e2, and return boo.tt if equal else boo.ff
+
+-- NOTATIONS
+notation b1 * b2 := conj b1 b2
+notation b1 + b2 := disj b1 b2
+prefix ! := neg
+
+-- REFACTOR INTO TEST FILE
+#reduce eval be4
+#reduce eval (conj (disj be2 be4) be3)
+#check X
+#check (var X)
+#reduce eval ((var X) * (var Y)) var_interp_1
+#reduce eval ((var X) * (var Y)) var_interp_2
+
+-- REFACTOR INTO TEST FILE
+#reduce eval ((be2 + be4) * be3)
+
+/-
+How do we know that eval terminates?
+-/
+
+-- Non-terminating functions would be fatal
+def bad : ℕ → false
+| n := bad n    -- non-terminating recursion
+#check (bad 3)  -- Yikes, a proof of false!
+
+-- PROPERTIES?
+
+/-
+A property of an expression, e, is that e
+evaluates to true. Let's call this property
+evaluates_to_true.
+-/
+def evaluates_to_true : bool_lang → Prop 
+| e := eval e = boo.tt
+/-
+This definition broke when we added an interpretation,
+i, as a second argument to eval.
+-/
+
+example : evaluates_to_true TT :=
+begin
+  unfold evaluates_to_true,
+  trivial,
+end
+--ditto last comment
+
+example : evaluates_to_true (TT * FF) :=
+begin
+  unfold evaluates_to_true,
+  simp [eval],
+  apply rfl,  -- false
+end
+--ditto last comment
+
+-- Property of an individual expression
+example : evaluates_to_true (TT * TT) :=
+begin
+  unfold evaluates_to_true,
+  simp [eval],
+  apply rfl,  -- false
+end
+--ditto last comment
+
+
+-- Property of the language as a whole: 
+-- evaluation is deterministic.
+
+-- HOMEWORK
+
+/-
+What deterministic means is that if you evaluate the same
+expression twice (in the same environment) that you'll get
+the same answer. A language with a statement that returns 
+a truly random number wouldn't have this property. Show that
+evaluation is deterministic for our "Bool" language.
+-/
+
+def eval_is_deterministic : 
+  ∀ (e : bool_lang) (i : bool_var → boo) (b1 b2 : boo), 
+  b1 = (eval e i) → 
+  b2 = (eval e i) → 
+  b1 = b2 := 
+begin
+  intros e i b1 b2 h1 h2,
+  rw h1,
+  rw h2,
+end
+
+
+def nat_eq : ℕ → ℕ → bool
+| nat.zero nat.zero := bool.tt
+| nat.zero _ := bool.ff
+| _ nat.zero := bool.ff
+| (nat.succ n') (nat.succ m') := nat_eq n' m'
+
+#reduce nat_eq 0 0
+#reduce nat_eq 0 1
+#reduce nat_eq 1 0
+#reduce nat_eq 1 1
+
+def var_eq : bool_var → bool_var → bool
+| (V n1) (V n2) := nat_eq n1 n2
+
+#reduce var_eq X X
+#reduce var_eq X Y
+#reduce var_eq X Z
+#reduce var_eq Y X
+#reduce var_eq Z X
+#reduce  var_eq Z Y
+#reduce var_eq Z Z
+
+def override : (bool_var → boo) → bool_var → boo → (bool_var → boo) :=
+λ i v' b, 
+  λ v, if (var_eq v v') then b else (i v)
+
+/-
+def var_interp_1 : bool_var → boo
+| v := boo.tt
+-/
+
+def init := var_interp_1
+
+#reduce init X
+#reduce init Y
+#reduce init Z
+
+def st_1 := override init X ff
+
+#reduce st_1 X
+#reduce st_1 Y
+#reduce st_1 Z
+
+def st_2 := override (st_1) Z ff
+
+#reduce st_2 X
+#reduce st_2 Y
+#reduce st_2 Z
+
+
+end arith
