src/content/project_1/arith_lang.lean
@@ -1,0 +1,87 @@
+import .nat
+
+namespace hidden 
+
+-- DATA TYPE
+
+inductive nt_var 
+| V (n : ℕ)
+
+open nt_var
+
+-- Test
+def X := V 0
+def Y := V 1
+def Z := V 2
+
+inductive nt_lang : Type
+| lit (n : nt)
+| var (v : nt_var) 
+| dec (e : nt_lang) 
+| inc (e : nt_lang) 
+| add (e1 e2 : nt_lang)
+
+
+-- REFACTOR INTO TEST FILE
+
+def init : nt_var → nt
+| v := nt.zero
+
+-- prefer to apply an override function
+def st_2 : nt_var → nt
+| (V 0) := one
+| _ := nt.zero
+
+-- OPERATIONS
+open nt_lang
+
+/-
+inductive nt_lang : Type
+| lit (n : nt)
+| var (v : nt_var) 
+| dec (e : nt_lang) 
+| inc (e : nt_lang) 
+| add (e1 e2 : nt_lang)
+-/
+
+def eval : nt_lang → (nt_var → nt) → nt
+| (lit n) _ := n
+| (var v) i := i v
+| (nt_lang.dec e) i := dec (eval e i)
+| (nt_lang.inc e) i := inc (eval e i)
+| (nt_lang.add e1 e2) i := add (eval e1 i) (eval e2 i)
+
+-- NOTATIONS
+notation e1 + e2 := add e1 e2
+
+
+/-
+def var_interp_1 : bool_var → boo
+| v := boo.tt
+-/
+
+/-
+-/
+
+def override : (nt_var → nt) → nt_var → nt → (nt_var → nt) :=
+λ i v n,
+  λ x, if (var_eq x v) then n else i x
+
+#reduce init X
+#reduce init Y
+#reduce init Z
+
+def st_1 := override init X ff
+
+#reduce st_1 X
+#reduce st_1 Y
+#reduce st_1 Z
+
+def st_2 := override (st_1) Z ff
+
+#reduce st_2 X
+#reduce st_2 Y
+#reduce st_2 Z
+
+
+end hidden
